use add and mul for the buffer length

code/frodo/Hacl.Impl.Frodo.fst
@@ -8,7 +8,6 @@ open Lib.IntTypes
 open Lib.RawIntTypes
 open Lib.PQ.Buffer
 open FStar.Mul
-open FStar.Math.Lemmas
 
 open Hacl.Impl.PQ.Lib
 open Hacl.Keccak
@@ -18,9 +17,7 @@ open LowStar.ModifiesPat
 open LowStar.Modifies
 
 module Buf = LowStar.Buffer
-module HS = FStar.HyperStack
 module ST = FStar.HyperStack.ST
-module Seq = FStar.Seq
 
 let cshake_frodo = cshake128_frodo
 
@@ -77,10 +74,12 @@ let lbytes_eq #len a b =
   pop_frame();
   res
 
-let bytes_mu =  normalize_term ((params_extracted_bits *. params_nbar *. params_nbar) /. size 8)
-let crypto_publickeybytes = normalize_term (bytes_seed_a +. (params_logq *. params_n *. params_nbar) /. size 8)
-let crypto_secretkeybytes = normalize_term (crypto_bytes +. crypto_publickeybytes +. size 2 *. params_n *. params_nbar)
-let crypto_ciphertextbytes = normalize_term (((params_nbar *. params_n +. params_nbar *. params_nbar) *. params_logq) /. size 8 +. crypto_bytes)
+let bytes_mu =  normalize_term ((params_extracted_bits *! params_nbar *! params_nbar) /. size 8)
+let crypto_publickeybytes = normalize_term (bytes_seed_a +! (params_logq *! params_n *! params_nbar) /. size 8)
+let crypto_secretkeybytes =
+  assert_norm (v crypto_bytes + v crypto_publickeybytes + 2 * v params_n * v params_nbar < max_size_t);
+  normalize_term (crypto_bytes +! crypto_publickeybytes +! size 2 *! params_n *! params_nbar)
+let crypto_ciphertextbytes = normalize_term (((params_nbar *! params_n +! params_nbar *! params_nbar) *! params_logq) /. size 8 +! crypto_bytes)
 
 #reset-options "--z3rlimit 50 --max_fuel 0"
 val ec:
@@ -97,8 +96,8 @@ let dc b c =
   res1 &. ((u16 1 <<. size_to_uint32 b) -. u16 1)
 
 val frodo_key_encode:
-  b:size_t{v ((params_nbar *. params_nbar *. b) /. size 8) < max_size_t /\ v b <= 8} ->
-  a:lbytes ((params_nbar *. params_nbar *. b) /. size 8) ->
+  b:size_t{v b <= 8} ->
+  a:lbytes ((params_nbar *! params_nbar *! b) /. size 8) ->
   res:matrix_t params_nbar params_nbar -> Stack unit
   (requires (fun h -> Buf.live h a /\ Buf.live h res /\ Buf.disjoint a res))
   (ensures (fun h0 _ h1 -> Buf.live h1 res /\ modifies (loc_buffer res) h0 h1))
@@ -106,7 +105,7 @@ val frodo_key_encode:
 let frodo_key_encode b a res =
   push_frame();
   let n2 = params_nbar /. size 8 in
-  let aLen = (params_nbar *. params_nbar *. b) /. size 8 in
+  let aLen = (params_nbar *! params_nbar *! b) /. size 8 in
   let v8 = create (size 8) (u8 0) in
   let h0 = ST.get () in
   let inv (h1:mem) (j:nat{j <= v params_nbar}) =
@@ -120,17 +119,17 @@ let frodo_key_encode b a res =
       let f1 (j:size_t{0 <= v j /\ v j < v n2}): Stack unit
         (requires (fun h -> inv1 h (v j)))
         (ensures (fun _ _ h2 -> inv1 h2 (v j + 1))) =
-          assume (v ((i +. j) *. b) + v b <= v aLen);
-          copy (sub v8 (size 0) b) b (sub #uint8 #(v aLen) #(v b) a ((i +. j) *. b) b);
+          assume ((v i + v j) * v b + v b <= v aLen);
+          copy (sub v8 (size 0) b) b (sub #uint8 #(v aLen) #(v b) a ((i +! j) *! b) b);
           let vij = uint_from_bytes_le #U64 v8 in
           let h1 = ST.get () in
           loop_nospec #h1 (size 8) res
           (fun k ->
-            assume (v (b *. k) < 64);
-            let ak = (vij >>. size_to_uint32 (b *. k)) &. ((u64 1 <<. size_to_uint32 b) -. u64 1) in
+            //assume (v (b *. k) < 64);
+            let ak = (vij >>. size_to_uint32 (b *! k)) &. ((u64 1 <<. size_to_uint32 b) -. u64 1) in
             let resij = ec b (to_u16 ak) in
-            assume (v (size 8 *. j +. k) < v params_nbar);
-            mset res i (size 8 *. j +. k) resij
+            assume (8 * v j + v k < v params_nbar);
+            mset res i (size 8 *! j +! k) resij
           ) in
 
       Lib.Loops.for (size 0) n2 inv1 f1 in
@@ -138,16 +137,16 @@ let frodo_key_encode b a res =
   pop_frame()
 
 val frodo_key_decode:
-  b:size_t{v ((params_nbar *. params_nbar *. b) /. size 8) < max_size_t /\ v b <= 8} ->
+  b:size_t{v b <= 8} ->
   a:matrix_t params_nbar params_nbar ->
-  res:lbytes ((params_nbar *. params_nbar *. b) /. size 8) -> Stack unit
+  res:lbytes ((params_nbar *! params_nbar *! b) /. size 8) -> Stack unit
   (requires (fun h -> Buf.live h a /\ Buf.live h res /\ Buf.disjoint a res))
   (ensures (fun h0 r h1 -> Buf.live h1 res /\ modifies (loc_buffer res) h0 h1))
   [@"c_inline"]
 let frodo_key_decode b a res =
   push_frame();
   let n2 = params_nbar /. size 8 in
-  let resLen = (params_nbar *. params_nbar *. b) /. size 8 in
+  let resLen = (params_nbar *! params_nbar *! b) /. size 8 in
   let v8 = create (size 8) (u8 0) in
   let templong:lbuffer uint64 1 = create (size 1) (u64 0) in
   let h0 = ST.get () in
@@ -168,14 +167,13 @@ let frodo_key_decode b a res =
           let h1 = ST.get () in
           loop_nospec #h1 (size 8) templong
           (fun k ->
-            assume (v (size 8 *. j +. k) < v params_nbar);
-            let aij = dc b (mget a i (size 8 *. j +. k)) in
-            assume (v (b *. k) < 64);
-            templong.(size 0) <- templong.(size 0) |. (to_u64 aij <<. size_to_uint32 (b *. k))
+            assume (8 * v j + v k < v params_nbar);
+            let aij = dc b (mget a i (size 8 *! j +! k)) in
+            templong.(size 0) <- templong.(size 0) |. (to_u64 aij <<. size_to_uint32 (b *! k))
           );
           uint_to_bytes_le #U64 v8 (templong.(size 0));
-          assume (v ((i +. j) *. b) + v b <= v resLen);
-          copy (sub res ((i +. j) *. b) b) b (sub #uint8 #8 #(v b) v8 (size 0) b) in
+          assume ((v i + v j) * v b + v b <= v resLen);
+          copy (sub res ((i +! j) *! b) b) b (sub #uint8 #8 #(v b) v8 (size 0) b) in
 
       Lib.Loops.for (size 0) n2 inv1 f1 in
   Lib.Loops.for (size 0) params_nbar inv f';
@@ -184,8 +182,8 @@ let frodo_key_decode b a res =
 val frodo_pack:
   n1:size_t -> n2:size_t{v n1 * v n2 < max_size_t /\ v n2 % 8 = 0} ->
   a:matrix_t n1 n2 ->
-  d:size_t{v ((d *. n1 *. n2) /. size 8) < max_size_t /\ v d <= 16} ->
-  res:lbytes ((d *. n1 *. n2) /. size 8) -> Stack unit
+  d:size_t{v d * v n1 < max_size_t /\ v d * v n1 * v n2 < max_size_t /\ v d <= 16} ->
+  res:lbytes (d *! n1 *! n2 /. size 8) -> Stack unit
   (requires (fun h -> Buf.live h a /\ Buf.live h res /\ Buf.disjoint a res))
   (ensures (fun h0 r h1 -> Buf.live h1 res /\ modifies (loc_buffer res) h0 h1))
   [@"c_inline"]
@@ -195,6 +193,7 @@ let frodo_pack n1 n2 a d res =
   let templong:lbuffer uint128 1 = create (size 1) (to_u128 (u64 0)) in
   let v16 = create (size 16) (u8 0) in
   let n28 = n2 /. size 8 in
+  let resLen = d *! n1 *! n2 /. size 8 in
 
   let h0 = ST.get () in
   let inv (h1:mem) (j:nat{j <= v n1}) =
@@ -214,14 +213,14 @@ let frodo_pack n1 n2 a d res =
           let h1 = ST.get () in
           loop_nospec #h1 (size 8) templong
           (fun k ->
-            assume (v (size 8 *. j +. k) < v n2);
-            let aij = to_u32 (mget a i (size 8 *. j +. k)) &. maskd in
-            assume (v (size 7 *. d -. d *. k) < 128);
-            templong.(size 0) <- templong.(size 0) |. (to_u128 aij <<. size_to_uint32 (size 7 *. d -. d *. k))
+            assume (8 * v j + v k < v n2);
+            let aij = to_u32 (mget a i (size 8 *! j +! k)) &. maskd in
+            //assume (v (size 7 *. d -. d *. k) < 128);
+            templong.(size 0) <- templong.(size 0) |. (to_u128 aij <<. size_to_uint32 (size 7 *! d -! d *! k))
           );
           uint_to_bytes_be #U128 v16 (templong.(size 0));
-          assume (v ((i *. n2 /. size 8 +. j) *. d) + v d <= v ((d *. n1 *. n2) /. size 8));
-          copy (sub res ((i *. n2 /. size 8 +. j) *. d) d) d (sub #uint8 #16 #(v d) v16 (size 16 -. d) d) in
+          assume (((v i * v n2 / 8 + v j) * v d) + v d <= v resLen);
+          copy (sub res ((i *! n2 /. size 8 +! j) *! d) d) d (sub #uint8 #16 #(v d) v16 (size 16 -! d) d) in
 
       Lib.Loops.for (size 0) n28 inv1 f1 in
   Lib.Loops.for (size 0) n1 inv f';
@@ -229,8 +228,8 @@ let frodo_pack n1 n2 a d res =
 
 val frodo_unpack:
   n1:size_t -> n2:size_t{v n1 * v n2 < max_size_t /\ v n2 % 8 = 0} ->
-  d:size_t{v ((d *. n1 *. n2) /. size 8) < max_size_t /\ v d <= 16} ->
-  b:lbytes ((d *. n1 *. n2) /. size 8) ->
+  d:size_t{v d * v n1 < max_size_t /\ v d * v n1 * v n2 < max_size_t /\ v d <= 16} ->
+  b:lbytes (d *! n1 *! n2 /. size 8) ->
   res:matrix_t n1 n2 -> Stack unit
   (requires (fun h -> Buf.live h b /\ Buf.live h res /\ Buf.disjoint b res))
   (ensures (fun h0 r h1 -> Buf.live h1 res /\ modifies (loc_buffer res) h0 h1))
@@ -238,8 +237,9 @@ val frodo_unpack:
 let frodo_unpack n1 n2 d b res =
   push_frame();
   let maskd = (u32 1 <<. size_to_uint32 d) -. u32 1 in
-  let v16 = create (size 16) (u8 0) in
+  let v16:lbytes (size 16) = create (size 16) (u8 0) in
   let n28 = n2 /. size 8 in
+  let bLen = d *! n1 *! n2 /. size 8 in
 
   let h0 = ST.get () in
   let inv (h1:mem) (j:nat{j <= v n1}) =
@@ -253,16 +253,18 @@ let frodo_unpack n1 n2 d b res =
       let f1 (j:size_t{0 <= v j /\ v j < v n28}): Stack unit
         (requires (fun h -> inv1 h (v j)))
         (ensures (fun _ _ h2 -> inv1 h2 (v j + 1))) =
-          assume (v ((i *. n28 +. j) *. d) + v d <= v ((d *. n1 *. n2) /. size 8));
-          copy (sub v16 (size 16 -. d) d) d (sub #uint8 #_ #(v d) b ((i *. n28 +. j) *. d) d);
+	  assume (v i * v n2 < max_size_t);
+	  assume ((v i * v n2 / 8 + v j) * v d < max_size_t);
+	  assume (v ((i *! n2 /. size 8 +! j) *! d) + v d <= v bLen);
+	  let bij = sub #_ #(v bLen) #(v d) b ((i *! n2 /. size 8 +! j) *! d) d in
+          copy (sub #_ #_ #(v d) v16 (size 16 -! d) d) d bij;
           let templong = uint_from_bytes_be #U128 v16 in
           let h1 = ST.get () in
-          loop_nospec #h1 (size 8) res // modifies res
+          loop_nospec #h1 (size 8) res
           (fun k ->
-            assume (v (size 7 *. d -. d *. k) < 128);
-            let resij = to_u32 (templong >>. size_to_uint32 (size 7 *. d -. d *. k)) &. maskd in
-            assume (v (size 8 *. j +. k) < v n2);
-            mset res i (size 8 *. j +. k) (to_u16 resij)
+            let resij = to_u32 (templong >>. size_to_uint32 (size 7 *! d -! d *! k)) &. maskd in
+            assume (8 * v j + v k < v n2);
+            mset res i (size 8 *! j +! k) (to_u16 resij)
           ) in
 
       Lib.Loops.for (size 0) n28 inv1 f1 in
@@ -278,7 +280,7 @@ let frodo_sample r =
   let prnd = r >>. u32 1 in
   let sign = r &. u16 1 in
   let sample:lbuffer uint16 1 = create (size 1) (u16 0) in
-  let ctr = cdf_table_len -. size 1 in
+  let ctr = cdf_table_len -! size 1 in
 
   let h0 = ST.get () in
   loop_nospec #h0 ctr sample
@@ -302,16 +304,16 @@ val frodo_sample_matrix:
   [@"c_inline"]
 let frodo_sample_matrix n1 n2 seed_len seed ctr res =
   push_frame();
-  let r = create (size 2 *. n1 *. n2) (u8 0) in
-  cshake_frodo seed_len seed ctr (size 2 *. n1 *. n2) r;
+  let r = create (size 2 *! n1 *! n2) (u8 0) in
+  cshake_frodo seed_len seed ctr (size 2 *! n1 *! n2) r;
   let h0 = ST.get () in
   loop_nospec #h0 n1 res
   (fun i ->
     let h0 = ST.get () in
     loop_nospec #h0 n2 res
     (fun j ->
-      assume (v (size 2 *. (n2 *. i +. j)) + 2 <= v (size 2 *. n1 *. n2));
-      let resij = sub r (size 2 *. (n2 *. i +. j)) (size 2) in
+      assume (2 * (v n2 * v i + v j) + 2 <= 2 * v n1 * v n2);
+      let resij = sub r (size 2 *! (n2 *! i +! j)) (size 2) in
       mset res i j (frodo_sample (uint_from_bytes_le #U16 resij))
     )
   );
@@ -326,16 +328,16 @@ val frodo_sample_matrix_tr:
   [@"c_inline"]
 let frodo_sample_matrix_tr n1 n2 seed_len seed ctr res =
   push_frame();
-  let r = create (size 2 *. n1 *. n2) (u8 0) in
-  cshake_frodo seed_len seed ctr (size 2 *. n1 *. n2) r;
+  let r = create (size 2 *! n1 *! n2) (u8 0) in
+  cshake_frodo seed_len seed ctr (size 2 *! n1 *! n2) r;
   let h0 = ST.get () in
   loop_nospec #h0 n1 res
   (fun i ->
     let h0 = ST.get () in
     loop_nospec #h0 n2 res
     (fun j ->
-      assume (v (size 2 *. (n1 *. j +. i)) + 2 <= v (size 2 *. n1 *. n2));
-      let resij = sub r (size 2 *. (n1 *. j +. i)) (size 2) in
+      assume (2 * (v n1 * v j + v i) + 2 <= 2 * v n1 * v n2);
+      let resij = sub r (size 2 *! (n1 *! j +! i)) (size 2) in
       mset res i j (frodo_sample (uint_from_bytes_le #U16 resij))
     )
   );
@@ -350,7 +352,7 @@ val frodo_gen_matrix_cshake:
   [@"c_inline"]
 let frodo_gen_matrix_cshake n seed_len seed res =
   push_frame();
-  let r:lbytes (size 2 *. n) = create (size 2 *. n) (u8 0) in
+  let r:lbytes (size 2 *! n) = create (size 2 *! n) (u8 0) in
   let h0 = ST.get () in
   let inv (h1:mem) (j:nat{j <= v n}) =
     Buf.live h1 res /\ Buf.live h1 r /\ modifies (loc_union (loc_buffer res) (loc_buffer r)) h0 h1 in
@@ -358,11 +360,11 @@ let frodo_gen_matrix_cshake n seed_len seed res =
     (requires (fun h -> inv h (v i)))
     (ensures (fun _ _ h2 -> inv h2 (v i + 1))) =
       let ctr = size_to_uint32 (size 256 +. i) in
-      cshake128_frodo seed_len seed (to_u16 ctr) (size 2 *. n) r;
+      cshake128_frodo seed_len seed (to_u16 ctr) (size 2 *! n) r;
       let h0 = ST.get () in
-      loop_nospec #h0 n res //modifies res
+      loop_nospec #h0 n res
       (fun j ->
-        let resij = sub r (size 2 *. j) (size 2) in
+        let resij = sub r (size 2 *! j) (size 2) in
         mset res i j (uint_from_bytes_le #U16 resij)
       ) in
   Lib.Loops.for (size 0) n inv f';
@@ -371,8 +373,8 @@ let frodo_gen_matrix_cshake n seed_len seed res =
 let frodo_gen_matrix = frodo_gen_matrix_cshake
 
 val matrix_to_lbytes:
-  #n1:size_t -> #n2:size_t{v n1 * v n2 < max_size_t} ->
-  m:matrix_t n1 n2 -> res:lbytes (size 2 *. n1 *. n2) -> Stack unit
+  #n1:size_t -> #n2:size_t{2 * v n1 < max_size_t /\ 2 * v n1 * v n2 < max_size_t} ->
+  m:matrix_t n1 n2 -> res:lbytes (size 2 *! n1 *! n2) -> Stack unit
   (requires (fun h -> Buf.live h m /\ Buf.live h res /\ Buf.disjoint m res))
   (ensures (fun h0 r h1 -> Buf.live h1 res /\ modifies (loc_buffer res) h0 h1))
   [@"c_inline"]
@@ -383,14 +385,14 @@ let matrix_to_lbytes #n1 #n2 m res =
     let h0 = ST.get () in
     loop_nospec #h0 n2 res
     (fun j ->
-      assume (v (size 2 *. (j *. n1 +. i)) + 2 <= v (size 2 *. n1 *. n2));
-      uint_to_bytes_le (sub res (size 2 *. (j *. n1 +. i)) (size 2)) (mget m i j)
+      assume (2 * (v j * v n1 + v i) + 2 <= 2 * v n1 * v n2);
+      uint_to_bytes_le (sub res (size 2 *! (j *! n1 +! i)) (size 2)) (mget m i j)
     )
   )
 
 val matrix_from_lbytes:
-  #n1:size_t -> #n2:size_t{v n1 * v n2 < max_size_t} ->
-  b:lbytes (size 2 *. n1 *. n2) ->
+  #n1:size_t -> #n2:size_t{2 * v n1 < max_size_t /\ 2 * v n1 * v n2 < max_size_t} ->
+  b:lbytes (size 2 *! n1 *! n2) ->
   res:matrix_t n1 n2 -> Stack unit
   (requires (fun h -> Buf.live h b /\ Buf.live h res /\ Buf.disjoint b res))
   (ensures (fun h0 r h1 -> Buf.live h1 res /\ modifies (loc_buffer res) h0 h1))
@@ -402,8 +404,8 @@ let matrix_from_lbytes #n1 #n2 b res =
     let h0 = ST.get () in
     loop_nospec #h0 n2 res
     (fun j ->
-      assume (v (size 2 *. (j *. n1 +. i)) + 2 <= v (size 2 *. n1 *. n2));
-      mset res i j (uint_from_bytes_le #U16 (sub b (size 2 *. (j *. n1 +. i)) (size 2)))
+      assume (2 * (v j * v n1 + v i) + 2 <= 2 * v n1 * v n2);
+      mset res i j (uint_from_bytes_le #U16 (sub b (size 2 *! (j *! n1 +! i)) (size 2)))
     )
   )
 
@@ -416,7 +418,6 @@ assume val randombytes_:
   len:size_t -> res:lbytes len -> Stack unit
   (requires (fun h -> Buf.live h res))
   (ensures (fun h0 r h1 -> Buf.live h1 res /\ modifies (loc_buffer res) h0 h1))
-
 
 val frodo_mul_add_as_plus_e:
   seed_a:lbytes bytes_seed_a ->
@@ -440,8 +441,8 @@ let frodo_mul_add_as_plus_e seed_a s_matrix e_matrix b_matrix =
 val frodo_mul_add_as_plus_e_pack:
   seed_a:lbytes bytes_seed_a ->
   seed_e:lbytes crypto_bytes ->
-  b:lbytes (params_logq *. params_n *. params_nbar /. size 8) ->
-  s:lbytes (size 2 *. params_n *. params_nbar) -> Stack unit
+  b:lbytes (params_logq *! params_n *! params_nbar /. size 8) ->
+  s:lbytes (size 2 *! params_n *! params_nbar) -> Stack unit
   (requires (fun h -> Buf.live h seed_a /\ Buf.live h seed_e /\
     Buf.live h s /\ Buf.live h b /\ Buf.disjoint b s /\
     Buf.disjoint seed_a b /\ Buf.disjoint seed_e b /\
@@ -463,24 +464,26 @@ let frodo_mul_add_as_plus_e_pack seed_a seed_e b s =
   pop_frame()
 
 val crypto_kem_keypair:
-  pk:lbytes crypto_publickeybytes{v (size 2 *. crypto_bytes +. bytes_seed_a) < max_size_t} ->
+  pk:lbytes crypto_publickeybytes ->
   sk:lbytes crypto_secretkeybytes -> Stack uint32
   (requires (fun h -> Buf.live h pk /\ Buf.live h sk /\ Buf.disjoint pk sk))
   (ensures (fun h0 r h1 -> Buf.live h1 pk /\ Buf.live h1 sk /\
     modifies (loc_union (loc_buffer pk) (loc_buffer sk)) h0 h1))
 let crypto_kem_keypair pk sk =
   push_frame();
-  let coins = create (size 2 *. crypto_bytes +. bytes_seed_a) (u8 0) in
-  randombytes_ (size 2 *. crypto_bytes +. bytes_seed_a) coins;
+  let coins = create (size 2 *! crypto_bytes +! bytes_seed_a) (u8 0) in
+  randombytes_ (size 2 *! crypto_bytes +! bytes_seed_a) coins;
   let s:lbytes crypto_bytes = sub coins (size 0) crypto_bytes in
   let seed_e = sub coins crypto_bytes crypto_bytes in
-  let z = sub coins (size 2 *. crypto_bytes) bytes_seed_a in
+  let z = sub coins (size 2 *! crypto_bytes) bytes_seed_a in
 
+  assert_norm (v crypto_publickeybytes = v bytes_seed_a + (v params_logq * v params_n * v params_nbar) / 8);
   let seed_a = sub pk (size 0) bytes_seed_a in
   cshake_frodo bytes_seed_a z (u16 0) bytes_seed_a seed_a;
 
-  let b:lbytes (params_logq *. params_n *. params_nbar /. size 8) = sub pk bytes_seed_a (crypto_publickeybytes -. bytes_seed_a) in
-  let s_matrix = sub sk (crypto_bytes +. crypto_publickeybytes) (size 2 *. params_n *. params_nbar) in
+  let b:lbytes (params_logq *! params_n *! params_nbar /. size 8) = sub pk bytes_seed_a (crypto_publickeybytes -! bytes_seed_a) in
+  assert_norm (v crypto_secretkeybytes = v crypto_bytes + v crypto_publickeybytes + 2 * v params_n * v params_nbar);
+  let s_matrix = sub sk (crypto_bytes +! crypto_publickeybytes) (size 2 *! params_n *! params_nbar) in
   frodo_mul_add_as_plus_e_pack seed_a seed_e b s_matrix;
 
   copy (sub sk (size 0) crypto_bytes) crypto_bytes s;
@@ -512,9 +515,9 @@ let frodo_mul_add_sa_plus_e seed_a seed_e sp_matrix bp_matrix =
   pop_frame()
 
 val frodo_mul_add_sb_plus_e_plus_mu:
-  b:lbytes ((params_logq *. params_n *. params_nbar) /. size 8) ->
+  b:lbytes ((params_logq *! params_n *! params_nbar) /. size 8) ->
   seed_e:lbytes crypto_bytes ->
-  coins:lbytes ((params_nbar *. params_nbar *. params_extracted_bits) /. size 8) ->
+  coins:lbytes ((params_nbar *! params_nbar *! params_extracted_bits) /. size 8) ->
   sp_matrix:matrix_t params_nbar params_n ->
   v_matrix:matrix_t params_nbar params_nbar -> Stack unit
   (requires (fun h -> Buf.live h b /\ Buf.live h seed_e /\
@@ -542,8 +545,8 @@ let frodo_mul_add_sb_plus_e_plus_mu b seed_e coins sp_matrix v_matrix =
 val crypto_kem_enc_ct_pack:
   seed_a:lbytes bytes_seed_a ->
   seed_e:lbytes crypto_bytes ->
-  coins:lbytes ((params_nbar *. params_nbar *. params_extracted_bits) /. size 8) ->
-  b:lbytes ((params_logq *. params_n *. params_nbar) /. size 8) ->
+  coins:lbytes ((params_nbar *! params_nbar *! params_extracted_bits) /. size 8) ->
+  b:lbytes ((params_logq *! params_n *! params_nbar) /. size 8) ->
   sp_matrix:matrix_t params_nbar params_n ->
   ct:lbytes crypto_ciphertextbytes -> Stack unit
   (requires (fun h -> Buf.live h seed_a /\ Buf.live h seed_e /\
@@ -553,11 +556,12 @@ val crypto_kem_enc_ct_pack:
   [@"c_inline"]
 let crypto_kem_enc_ct_pack seed_a seed_e coins b sp_matrix ct =
   push_frame();
-  let c1Len = (params_logq *. params_nbar *. params_n) /. size 8 in
-  let c2Len = (params_logq *. params_nbar *. params_nbar) /. size 8 in
+  let c1Len = (params_logq *! params_nbar *! params_n) /. size 8 in
+  let c2Len = (params_logq *! params_nbar *! params_nbar) /. size 8 in
 
   let bp_matrix = matrix_create params_nbar params_n in
   frodo_mul_add_sa_plus_e seed_a seed_e sp_matrix bp_matrix;
+  assert_norm (v crypto_ciphertextbytes = ((v params_nbar * v params_n + v params_nbar * v params_nbar) * v params_logq) / 8 + v crypto_bytes);
   frodo_pack params_nbar params_n bp_matrix params_logq (sub ct (size 0) c1Len);
 
   let v_matrix   = matrix_create params_nbar params_nbar in
@@ -567,8 +571,8 @@ let crypto_kem_enc_ct_pack seed_a seed_e coins b sp_matrix ct =
 
 val crypto_kem_enc_ct:
   pk:lbytes crypto_publickeybytes ->
-  g:lbytes (size 3 *. crypto_bytes){3 * v crypto_bytes < max_size_t} ->
-  coins:lbytes ((params_nbar *. params_nbar *. params_extracted_bits) /. size 8) ->
+  g:lbytes (size 3 *! crypto_bytes){3 * v crypto_bytes < max_size_t} ->
+  coins:lbytes ((params_nbar *! params_nbar *! params_extracted_bits) /. size 8) ->
   ct:lbytes crypto_ciphertextbytes -> Stack unit
   (requires (fun h -> Buf.live h pk /\ Buf.live h g /\
     Buf.live h coins /\ Buf.live h ct /\ Buf.disjoint g ct /\
@@ -577,22 +581,24 @@ val crypto_kem_enc_ct:
   [@"c_inline"]
 let crypto_kem_enc_ct pk g coins ct =
   push_frame();
-  let c1Len = (params_logq *. params_nbar *. params_n) /. size 8 in
-  let c2Len = (params_logq *. params_nbar *. params_nbar) /. size 8 in
-  let c12Len = c1Len +. c2Len in
+  assert_norm (v crypto_ciphertextbytes = ((v params_nbar * v params_n + v params_nbar * v params_nbar) * v params_logq) / 8 + v crypto_bytes);
+  assert_norm (v crypto_publickeybytes = v bytes_seed_a + (v params_logq * v params_n * v params_nbar) / 8);
+  let c1Len = (params_logq *! params_nbar *! params_n) /. size 8 in
+  let c2Len = (params_logq *! params_nbar *! params_nbar) /. size 8 in
+  let c12Len = c1Len +! c2Len in
   let seed_a = sub #uint8 #_ #(v bytes_seed_a) pk (size 0) bytes_seed_a in
   let seed_e = sub #uint8 #_ #(v crypto_bytes) g (size 0) crypto_bytes in
-  let b = sub #uint8 #_ #(v ((params_logq *. params_n *. params_nbar) /. size 8)) pk bytes_seed_a (crypto_publickeybytes -. bytes_seed_a) in
+  let b = sub #uint8 #_ #(v ((params_logq *! params_n *! params_nbar) /. size 8)) pk bytes_seed_a (crypto_publickeybytes -! bytes_seed_a) in
   let sp_matrix = matrix_create params_nbar params_n in
   frodo_sample_matrix params_nbar params_n crypto_bytes seed_e (u16 4) sp_matrix;
 
   crypto_kem_enc_ct_pack seed_a seed_e coins b sp_matrix ct;
-  let d = sub #uint8 #_ #(v crypto_bytes) g (size 2 *.crypto_bytes) crypto_bytes in
+  let d = sub #uint8 #_ #(v crypto_bytes) g (size 2 *! crypto_bytes) crypto_bytes in
   copy (sub ct c12Len crypto_bytes) crypto_bytes d;
   pop_frame()
 
 val crypto_kem_enc_ss:
-  g:lbytes (size 3 *. crypto_bytes) ->
+  g:lbytes (size 3 *! crypto_bytes) ->
   ct:lbytes crypto_ciphertextbytes ->
   ss:lbytes crypto_bytes -> Stack unit
   (requires (fun h -> Buf.live h g /\ Buf.live h ct /\ Buf.live h ss /\
@@ -601,18 +607,19 @@ val crypto_kem_enc_ss:
   [@"c_inline"]
 let crypto_kem_enc_ss g ct ss =
   push_frame();
-  let c1Len = (params_logq *. params_nbar *. params_n) /. size 8 in
-  let c2Len = (params_logq *. params_nbar *. params_nbar) /. size 8 in
-  let c12Len = c1Len +. c2Len in
-  let ss_init_len = c12Len +. size 2 *. crypto_bytes in
+  assert_norm (v crypto_ciphertextbytes = ((v params_nbar * v params_n + v params_nbar * v params_nbar) * v params_logq) / 8 + v crypto_bytes);
+  let c1Len = (params_logq *! params_nbar *! params_n) /. size 8 in
+  let c2Len = (params_logq *! params_nbar *! params_nbar) /. size 8 in
+  let c12Len = c1Len +! c2Len in
+  let ss_init_len = c12Len +! size 2 *! crypto_bytes in
   let ss_init:lbytes ss_init_len = create ss_init_len (u8 0) in
 
   let k = sub #uint8 #_ #(v crypto_bytes) g crypto_bytes crypto_bytes in
-  let d = sub #uint8 #_ #(v crypto_bytes) g (size 2 *. crypto_bytes) crypto_bytes in
+  let d = sub #uint8 #_ #(v crypto_bytes) g (size 2 *! crypto_bytes) crypto_bytes in
 
   copy (sub ss_init (size 0) c12Len) c12Len (sub #uint8 #_ #(v c12Len) ct (size 0) c12Len);
   copy (sub ss_init c12Len crypto_bytes) crypto_bytes k;
-  copy (sub ss_init (ss_init_len -. crypto_bytes) crypto_bytes) crypto_bytes d;
+  copy (sub ss_init (ss_init_len -! crypto_bytes) crypto_bytes) crypto_bytes d;
   cshake_frodo ss_init_len ss_init (u16 7) crypto_bytes ss;
   pop_frame()
 
@@ -625,38 +632,39 @@ val crypto_kem_enc:
     modifies (loc_union (loc_buffer ct) (loc_buffer ss)) h0 h1))
 let crypto_kem_enc ct ss pk =
   push_frame();
+  assert_norm (v crypto_ciphertextbytes = ((v params_nbar * v params_n + v params_nbar * v params_nbar) * v params_logq) / 8 + v crypto_bytes);
+  assert_norm (v crypto_publickeybytes = v bytes_seed_a + (v params_logq * v params_n * v params_nbar) / 8);
   assert_norm (v bytes_mu = v ((params_nbar *. params_nbar *. params_extracted_bits) /. size 8));
 
-  let coins = create ((params_nbar *. params_nbar *. params_extracted_bits) /. size 8) (u8 0) in
-  randombytes_ ((params_nbar *. params_nbar *. params_extracted_bits) /. size 8) coins;
+  let coins = create ((params_nbar *! params_nbar *! params_extracted_bits) /. size 8) (u8 0) in
+  randombytes_ ((params_nbar *! params_nbar *! params_extracted_bits) /. size 8) coins;
 
-  assert_norm (v crypto_bytes + v bytes_mu < max_size_t);
-  let pk_coins = create (crypto_publickeybytes +. bytes_mu) (u8 0) in
+  let pk_coins = create (crypto_publickeybytes +! bytes_mu) (u8 0) in
   copy (sub pk_coins (size 0) crypto_publickeybytes) crypto_publickeybytes pk;
   copy (sub pk_coins crypto_publickeybytes bytes_mu) bytes_mu coins;
-  assert_norm (3 * v crypto_bytes < max_size_t);
-  let g:lbytes (size 3 *. crypto_bytes) = create (size 3 *. crypto_bytes) (u8 0) in
-  cshake_frodo (crypto_publickeybytes +. bytes_mu) pk_coins (u16 3) (size 3 *. crypto_bytes) g;
+
+  let g:lbytes (size 3 *! crypto_bytes) = create (size 3 *! crypto_bytes) (u8 0) in
+  cshake_frodo (crypto_publickeybytes +! bytes_mu) pk_coins (u16 3) (size 3 *! crypto_bytes) g;
 
   crypto_kem_enc_ct pk g coins ct;
   crypto_kem_enc_ss g ct ss;
   pop_frame();
   (u32 0)
 
-
 val frodo_sub_mul_c_minus_bs:
   sk:lbytes crypto_secretkeybytes ->
   bp_matrix:matrix_t params_nbar params_n ->
   c_matrix:matrix_t params_nbar params_nbar ->
-  mu_decode:lbytes (params_nbar *. params_nbar *. params_extracted_bits /. size 8) -> Stack unit
+  mu_decode:lbytes (params_nbar *! params_nbar *! params_extracted_bits /. size 8) -> Stack unit
   (requires (fun h -> Buf.live h sk /\ Buf.live h bp_matrix /\
     Buf.live h c_matrix /\ Buf.live h mu_decode))
   (ensures (fun h0 r h1 -> Buf.live h1 mu_decode /\ modifies (loc_buffer mu_decode) h0 h1))
   [@"c_inline"]
 let frodo_sub_mul_c_minus_bs sk bp_matrix c_matrix mu_decode =
   push_frame();
+  assert_norm (v crypto_secretkeybytes = v crypto_bytes + v crypto_publickeybytes + 2 * v params_n * v params_nbar);
   let s_matrix  = matrix_create params_n params_nbar in
-  matrix_from_lbytes (sub sk (crypto_bytes +. crypto_publickeybytes) (size 2 *. params_n *. params_nbar)) s_matrix;
+  matrix_from_lbytes (sub sk (crypto_bytes +! crypto_publickeybytes) (size 2 *! params_n *! params_nbar)) s_matrix;
 
   let m_matrix  = matrix_create params_nbar params_nbar in
   matrix_mul bp_matrix s_matrix m_matrix;
@@ -667,7 +675,7 @@ let frodo_sub_mul_c_minus_bs sk bp_matrix c_matrix mu_decode =
 
 val crypto_kem_dec_ss:
   ct:lbytes crypto_ciphertextbytes ->
-  g:lbytes (size 3 *. crypto_bytes) ->
+  g:lbytes (size 3 *! crypto_bytes) ->
   kp_s:lbytes crypto_bytes ->
   ss:lbytes crypto_bytes -> Stack unit
   (requires (fun h -> Buf.live h ct /\ Buf.live h g /\
@@ -677,48 +685,56 @@ val crypto_kem_dec_ss:
   [@"c_inline"]
 let crypto_kem_dec_ss ct g kp_s ss =
   push_frame();
-  let c1Len = (params_logq *. params_nbar *. params_n) /. size 8 in
-  let c2Len = (params_logq *. params_nbar *. params_nbar) /. size 8 in
+  assert_norm (v crypto_ciphertextbytes = ((v params_nbar * v params_n + v params_nbar * v params_nbar) * v params_logq) / 8 + v crypto_bytes);
+  let c1Len = (params_logq *! params_nbar *! params_n) /. size 8 in
+  let c2Len = (params_logq *! params_nbar *! params_nbar) /. size 8 in
   let c1 = sub #uint8 #_ #(v c1Len) ct (size 0) c1Len in
   let c2 = sub #uint8 #_ #(v c2Len) ct c1Len c2Len in
-  let d = sub #uint8 #_ #(v crypto_bytes) ct (c1Len +. c2Len) crypto_bytes in
+  let d = sub #uint8 #_ #(v crypto_bytes) ct (c1Len +! c2Len) crypto_bytes in
 
-  let ss_init_len = c1Len +. c2Len +. size 2 *. crypto_bytes in
+  let ss_init_len = c1Len +! c2Len +! size 2 *! crypto_bytes in
   let ss_init:lbytes ss_init_len = create ss_init_len (u8 0) in
   copy (sub ss_init (size 0) c1Len) c1Len c1;
   copy (sub ss_init c1Len c2Len) c2Len c2;
-  copy (sub ss_init (c1Len +. c2Len) crypto_bytes) crypto_bytes kp_s;
-  copy (sub ss_init (ss_init_len -. crypto_bytes) crypto_bytes) crypto_bytes d;
-  
+  copy (sub ss_init (c1Len +! c2Len) crypto_bytes) crypto_bytes kp_s;
+  copy (sub ss_init (ss_init_len -! crypto_bytes) crypto_bytes) crypto_bytes d;
+
   cshake_frodo ss_init_len ss_init (u16 7) crypto_bytes ss;
   pop_frame()
 
+let pk_mu_decode_len =
+  assert_norm (v crypto_publickeybytes + v params_nbar * v params_nbar * v params_extracted_bits / 8 < max_size_t);
+  normalize_term (crypto_publickeybytes +! params_nbar *! params_nbar *! params_extracted_bits /. size 8)
 
 val crypto_kem_dec_ss1:
-  pk_mu_decode:lbytes (crypto_publickeybytes +. params_nbar *. params_nbar *. params_extracted_bits /. size 8) ->
+  pk_mu_decode:lbytes pk_mu_decode_len ->
   bp_matrix:matrix_t params_nbar params_n ->
   c_matrix:matrix_t params_nbar params_nbar ->
   sk:lbytes crypto_secretkeybytes ->
   ct:lbytes crypto_ciphertextbytes ->
   ss:lbytes crypto_bytes -> Stack unit
   (requires (fun h -> Buf.live h pk_mu_decode /\ Buf.live h bp_matrix /\
-    Buf.live h c_matrix /\ Buf.live h sk /\ Buf.live h ct /\ 
+    Buf.live h c_matrix /\ Buf.live h sk /\ Buf.live h ct /\
     Buf.live h ss /\ Buf.disjoint ss ct /\ Buf.disjoint ss sk))
   (ensures (fun h0 r h1 -> Buf.live h1 ss /\ modifies (loc_buffer ss) h0 h1))
   [@"c_inline"]
 let crypto_kem_dec_ss1 pk_mu_decode bp_matrix c_matrix sk ct ss =
   push_frame();
+  assert_norm (v crypto_ciphertextbytes = ((v params_nbar * v params_n + v params_nbar * v params_nbar) * v params_logq) / 8 + v crypto_bytes);
+  assert_norm (v crypto_secretkeybytes = v crypto_bytes + v crypto_publickeybytes + 2 * v params_n * v params_nbar);
+  assert_norm (v crypto_publickeybytes = v bytes_seed_a + (v params_logq * v params_n * v params_nbar) / 8);
+  assert_norm (v pk_mu_decode_len = v crypto_publickeybytes + v params_nbar * v params_nbar * v params_extracted_bits / 8);
   let s = sub #uint8 #_ #(v crypto_bytes) sk (size 0) crypto_bytes in
   let pk = sub #uint8 #_ #(v crypto_publickeybytes) sk crypto_bytes crypto_publickeybytes in
   let seed_a = sub #uint8 #_ #(v bytes_seed_a) pk (size 0) bytes_seed_a in
-  let b = sub #uint8 #_ #(v ((params_logq *. params_n *. params_nbar) /. size 8)) pk bytes_seed_a (crypto_publickeybytes -. bytes_seed_a) in
-  
-  let mu_decode_len = params_nbar *. params_nbar *. params_extracted_bits /. size 8 in
-  let g = create (size 3 *. crypto_bytes) (u8 0) in
-  cshake_frodo (crypto_publickeybytes +. mu_decode_len) pk_mu_decode (u16 3) (size 3 *. crypto_bytes) g;
+  let b = sub #uint8 #_ #(v ((params_logq *! params_n *! params_nbar) /. size 8)) pk bytes_seed_a (crypto_publickeybytes -! bytes_seed_a) in
+
+  let mu_decode_len = params_nbar *! params_nbar *! params_extracted_bits /. size 8 in
+  let g = create (size 3 *! crypto_bytes) (u8 0) in
+  cshake_frodo (crypto_publickeybytes +! mu_decode_len) pk_mu_decode (u16 3) (size 3 *! crypto_bytes) g;
   let seed_ep = sub #uint8 #_ #(v crypto_bytes) g (size 0) crypto_bytes in
-  let kp = sub #uint8 #_ #(v crypto_bytes) g crypto_bytes crypto_bytes in  
-  let dp = sub #uint8 #_ #(v crypto_bytes) g (size 2 *. crypto_bytes) crypto_bytes in
+  let kp = sub #uint8 #_ #(v crypto_bytes) g crypto_bytes crypto_bytes in
+  let dp = sub #uint8 #_ #(v crypto_bytes) g (size 2 *! crypto_bytes) crypto_bytes in
 
   let sp_matrix  = matrix_create params_nbar params_n in
   frodo_sample_matrix params_nbar params_n crypto_bytes seed_ep (u16 4) sp_matrix;
@@ -727,12 +743,12 @@ let crypto_kem_dec_ss1 pk_mu_decode bp_matrix c_matrix sk ct ss =
   frodo_mul_add_sa_plus_e seed_a seed_ep sp_matrix bpp_matrix;
 
   let v_matrix   = matrix_create params_nbar params_nbar in
-  let mu_decode  = sub pk_mu_decode crypto_publickeybytes (params_nbar *. params_nbar *. params_extracted_bits /. size 8) in
+  let mu_decode  = sub pk_mu_decode crypto_publickeybytes (params_nbar *! params_nbar *! params_extracted_bits /. size 8) in
   frodo_mul_add_sb_plus_e_plus_mu b seed_ep mu_decode sp_matrix v_matrix;
 
-  let c1Len = (params_logq *. params_nbar *. params_n) /. size 8 in
-  let c2Len = (params_logq *. params_nbar *. params_nbar) /. size 8 in
-  let d = sub #uint8 #_ #(v crypto_bytes) ct (c1Len +. c2Len) crypto_bytes in
+  let c1Len = (params_logq *! params_nbar *! params_n) /. size 8 in
+  let c2Len = (params_logq *! params_nbar *! params_nbar) /. size 8 in
+  let d = sub #uint8 #_ #(v crypto_bytes) ct (c1Len +! c2Len) crypto_bytes in
   let b1 = lbytes_eq d dp in
   let b2 = matrix_eq params_logq bp_matrix bpp_matrix in
   let b3 = matrix_eq params_logq c_matrix v_matrix in
@@ -748,24 +764,28 @@ val crypto_kem_dec:
   (ensures (fun h0 r h1 -> Buf.live h1 ss /\ modifies (loc_buffer ss) h0 h1))
 let crypto_kem_dec ss ct sk =
   push_frame();
-  let c1Len = (params_logq *. params_nbar *. params_n) /. size 8 in
-  let c2Len = (params_logq *. params_nbar *. params_nbar) /. size 8 in
+  assert_norm (v crypto_ciphertextbytes = ((v params_nbar * v params_n + v params_nbar * v params_nbar) * v params_logq) / 8 + v crypto_bytes);
+  assert_norm (v crypto_secretkeybytes = v crypto_bytes + v crypto_publickeybytes + 2 * v params_n * v params_nbar);
+  assert_norm (v crypto_publickeybytes = v bytes_seed_a + (v params_logq * v params_n * v params_nbar) / 8);
+  assert_norm (v pk_mu_decode_len = v crypto_publickeybytes + v params_nbar * v params_nbar * v params_extracted_bits / 8);
+  
+  let c1Len = (params_logq *! params_nbar *! params_n) /. size 8 in
+  let c2Len = (params_logq *! params_nbar *! params_nbar) /. size 8 in
   let c1 = sub #uint8 #_ #(v c1Len) ct (size 0) c1Len in
   let c2 = sub #uint8 #_ #(v c2Len) ct c1Len c2Len in
-  let d = sub #uint8 #_ #(v crypto_bytes) ct (c1Len +. c2Len) crypto_bytes in
-  
+  let d = sub #uint8 #_ #(v crypto_bytes) ct (c1Len +! c2Len) crypto_bytes in
+
   let bp_matrix = matrix_create params_nbar params_n in
   let c_matrix  = matrix_create params_nbar params_nbar in
   frodo_unpack params_nbar params_n params_logq c1 bp_matrix;
   frodo_unpack params_nbar params_nbar params_logq c2 c_matrix;
 
-  let mu_decode_len = params_nbar *. params_nbar *. params_extracted_bits /. size 8 in
-  let mu_decode = create (params_nbar *. params_nbar *. params_extracted_bits /. size 8) (u8 0) in
+  let mu_decode_len = params_nbar *! params_nbar *! params_extracted_bits /. size 8 in
+  let mu_decode = create (params_nbar *! params_nbar *! params_extracted_bits /. size 8) (u8 0) in
   frodo_sub_mul_c_minus_bs sk bp_matrix c_matrix mu_decode;
 
-  assert_norm (v crypto_publickeybytes + v mu_decode_len < max_size_t);
-  let pk_mu_decode = create (crypto_publickeybytes +. mu_decode_len) (u8 0) in
-  let pk = sub #uint8 #_ #(v crypto_publickeybytes) sk crypto_bytes crypto_publickeybytes in  
+  let pk_mu_decode = create (crypto_publickeybytes +! mu_decode_len) (u8 0) in
+  let pk = sub #uint8 #_ #(v crypto_publickeybytes) sk crypto_bytes crypto_publickeybytes in
   copy (sub pk_mu_decode (size 0) crypto_publickeybytes) crypto_publickeybytes pk;
   copy (sub #_ #(v crypto_publickeybytes + v mu_decode_len) #(v mu_decode_len) pk_mu_decode crypto_publickeybytes mu_decode_len) mu_decode_len mu_decode;
 
